{-# OPTIONS --without-K #-}

open import lib.Base
open import lib.PathGroupoid
open import lib.PathFunctor
open import lib.NType

module lib.Equivalences where

{-
We use the half-adjoint definition of equivalences (but this fact should be
invisible to the user of the library). The constructor of the type of
equivalences is [equiv], it takes two maps and the two proofs that the composites
are equal: [equiv to from to-from from-to]

The type of equivalences between two types [A] and [B] can be written either
[A ≃ B] or [Equiv A B].

Given an equivalence [e] : [A ≃ B], you can extract the two maps as follows:
[–> e] : [A → B] and [<– e] : [B → A] (the dash is an en dash)
The proofs that the composites are the identities are [<–-inv-l] and [<–-inv-r].

The identity equivalence on [A] is [ide A], the composition of two equivalences
is [_∘e_] (function composition order) and the inverse of an equivalence is [_⁻¹]
-}

module _ {i} {j} {A : Type i} {B : Type j} where

  record is-equiv (f : A → B) : Type (lmax i j)
    where
    field
      g : B → A
      f-g : (b : B) → f (g b) == b
      g-f : (a : A) → g (f a) == a
      adj : (a : A) → ap f (g-f a) == f-g (f a)

  {-
  In order to prove that something is an equivalence, you have to give an inverse
  and a proof that it’s an inverse (you don’t need the adj part).
  [is-eq] is a very, very bad name.
  -}
  is-eq : (f : A → B)
    (g : B → A) (f-g : (b : B) → f (g b) == b)
    (g-f : (a : A) → g (f a) == a) → is-equiv f
  is-eq f g f-g g-f =
   record {g = g; f-g = f-g'; g-f = g-f; adj = adj} where
    f-g' : (b : B) → f (g b) == b
    f-g' b = ! (ap (f ∘ g) (f-g b)) ∙ ap f (g-f (g b)) ∙ f-g b

    adj : (a : A) → ap f (g-f a) == f-g' (f a)
    adj a = 
      ap f (g-f a)
        =⟨ ! (!-inv-l (ap (f ∘ g) (f-g (f a)))) |in-ctx (λ q → q ∙ ap f (g-f a)) ⟩
      (! (ap (f ∘ g) (f-g (f a))) ∙ ap (f ∘ g) (f-g (f a))) ∙ ap f (g-f a)
        =⟨ ∙-assoc (! (ap (f ∘ g) (f-g (f a)))) (ap (f ∘ g) (f-g (f a))) _ ⟩
      ! (ap (f ∘ g) (f-g (f a))) ∙ ap (f ∘ g) (f-g (f a)) ∙ ap f (g-f a)
        =⟨ lemma |in-ctx (λ q → ! (ap (f ∘ g) (f-g (f a))) ∙ q) ⟩
      ! (ap (f ∘ g) (f-g (f a))) ∙ ap f (g-f (g (f a))) ∙ f-g (f a) ∎ 
      where 
      lemma : ap (f ∘ g) (f-g (f a)) ∙ ap f (g-f a) 
           == ap f (g-f (g (f a))) ∙ f-g (f a)
      lemma = 
        ap (f ∘ g) (f-g (f a)) ∙ ap f (g-f a)
          =⟨ htpy-natural-toid f-g (f a) |in-ctx (λ q → q ∙ ap f (g-f a)) ⟩
        f-g (f (g (f a))) ∙ ap f (g-f a)
          =⟨ ! (ap-idf (ap f (g-f a))) |in-ctx (λ q → f-g (f (g (f a))) ∙ q) ⟩
        f-g (f (g (f a))) ∙ ap (idf B) (ap f (g-f a))
          =⟨ ! (htpy-natural f-g (ap f (g-f a))) ⟩
        ap (f ∘ g) (ap f (g-f a)) ∙ f-g (f a)
          =⟨ ap-∘ f g (ap f (g-f a)) |in-ctx (λ q → q ∙ f-g (f a)) ⟩
        ap f (ap g (ap f (g-f a))) ∙ f-g (f a)
          =⟨ ∘-ap g f (g-f a) ∙ htpy-natural-toid g-f a 
             |in-ctx (λ q → ap f q ∙ f-g (f a)) ⟩
        ap f (g-f (g (f a))) ∙ f-g (f a) ∎

_≃_ : ∀ {i j} (A : Type i) (B : Type j) → Type (lmax i j)
A ≃ B = Σ (A → B) is-equiv

Equiv = _≃_

module _ {i} {j} {A : Type i} {B : Type j} where

  equiv : (f : A → B) (g : B → A) (f-g : (b : B) → f (g b) == b)
          (g-f : (a : A) → g (f a) == a) → A ≃ B
  equiv f g f-g g-f = (f , is-eq f g f-g g-f)

  –> : (e : A ≃ B) → (A → B)
  –> e = fst e

  <– : (e : A ≃ B) → (B → A)
  <– e = is-equiv.g (snd e)

  <–-inv-l : (e : A ≃ B) (a : A)
    → (<– e (–> e a) == a)
  <–-inv-l e a = is-equiv.g-f (snd e) a

  <–-inv-r : (e : A ≃ B) (b : B)
    → (–> e (<– e b) == b)
  <–-inv-r e b = is-equiv.f-g (snd e) b

  -- Equivalences are "injective"
  equiv-inj : (e : A ≃ B) {x y : A}
    → (–> e x == –> e y → x == y)
  equiv-inj e {x} {y} p = ! (<–-inv-l e x) ∙ ap (<– e) p ∙ <–-inv-l e y

idf-is-equiv : ∀ {i} (A : Type i) → is-equiv (idf A)
idf-is-equiv A = is-eq _ (idf A) (λ _ → idp) (λ _ → idp)

ide : ∀ {i} (A : Type i) → A ≃ A
ide A = equiv (idf A) (idf A) (λ _ → idp) (λ _ → idp)

infixr 4 _∘e_
infixr 4 _∘ise_

_∘e_ : ∀ {i j k} {A : Type i} {B : Type j} {C : Type k}
  → B ≃ C → A ≃ B → A ≃ C
e1 ∘e e2 = equiv (–> e1 ∘ –> e2) (<– e2 ∘ <– e1)
  (λ c → –> e1 (–> e2 (<– e2 (<– e1 c)))
                   =⟨ <–-inv-r e2 (<– e1 c) |in-ctx (–> e1) ⟩
         –> e1 (<– e1 c)  =⟨ <–-inv-r e1 c ⟩
         c ∎)
  (λ a → <– e2 (<– e1 (–> e1 (–> e2 a)))
                   =⟨ <–-inv-l e1 (–> e2 a) |in-ctx (<– e2) ⟩
         <– e2 (–> e2 a)  =⟨ <–-inv-l e2 a ⟩
         a ∎)

_∘ise_ : ∀ {i j k} {A : Type i} {B : Type j} {C : Type k}
  {f : A → B} {g : B → C}
  → is-equiv g → is-equiv f → is-equiv (g ∘ f)
i1 ∘ise i2 = snd ((_ , i1) ∘e (_ , i2))

_⁻¹ : ∀ {i j} {A : Type i} {B : Type j} → (A ≃ B) → (B ≃ A)
e ⁻¹ = equiv (<– e) (–> e) (<–-inv-l e) (<–-inv-r e)

{- Equational reasoning for equivalences -}
infix  2 _≃∎
infixr 2 _≃⟨_⟩_

_≃⟨_⟩_ : ∀ {i j k} (A : Type i) {B : Type j} {C : Type k} → A ≃ B → B ≃ C → A ≃ C
A ≃⟨ u ⟩ v = v ∘e u

_≃∎ : ∀ {i} (A : Type i) → A ≃ A
_≃∎ = ide

{- Any contractible type is equivalent to all liftings of the unit type -}
contr-equiv-LiftUnit : ∀ {i j} {A : Type i} → (is-contr A → A ≃ Lift {j = j} Unit)
contr-equiv-LiftUnit e =
  equiv (λ _ → lift unit) (λ _ → fst e) (λ _ → idp) (λ a → snd e a)


{- An equivalence induces an equivalence on the path spaces -}
module _ {i j} {A : Type i} {B : Type j} (e : A ≃ B) where

  private
    abstract
      left-inverse : {x y : A} (p : x == y) → equiv-inj e (ap (–> e) p) == p
      left-inverse idp = !-inv-l (<–-inv-l e _)

      right-inverse : {x y : A} (p : –> e x == –> e y) 
        → ap (–> e) (equiv-inj e p) == p
      right-inverse {x} {y} p = 
        ap f (! (g-f x) ∙ ap g p ∙ (g-f y))
          =⟨ ap-∙ f (! (g-f x)) (ap g p ∙ (g-f y)) ⟩
        ap f (! (g-f x)) ∙ ap f (ap g p ∙ (g-f y))
          =⟨ ap-∙ f (ap g p) (g-f y) |in-ctx (λ q →  ap f (! (g-f x)) ∙ q) ⟩
        ap f (! (g-f x)) ∙ ap f (ap g p) ∙ ap f (g-f y)
          =⟨ ∘-ap f g p |in-ctx (λ q → ap f (! (g-f x)) ∙ q ∙ ap f (g-f y)) ⟩
        ap f (! (g-f x)) ∙ ap (f ∘ g) p ∙ ap f (g-f y)
          =⟨ adj y |in-ctx (λ q →  ap f (! (g-f x)) ∙ ap (f ∘ g) p ∙ q) ⟩
        ap f (! (g-f x)) ∙ ap (f ∘ g) p ∙ (f-g (f y))
          =⟨ ap-! f (g-f x) |in-ctx (λ q → q ∙ ap (f ∘ g) p ∙ (f-g (f y))) ⟩
        ! (ap f (g-f x)) ∙ ap (f ∘ g) p ∙ (f-g (f y))
          =⟨ adj x |in-ctx (λ q →  ! q ∙ ap (f ∘ g) p ∙ (f-g (f y))) ⟩
        ! (f-g (f x)) ∙ ap (f ∘ g) p ∙ (f-g (f y))
          =⟨ htpy-natural f-g p |in-ctx (λ q →  ! (f-g (f x)) ∙ q) ⟩
        ! (f-g (f x)) ∙ (f-g (f x)) ∙ ap (idf B) p
          =⟨ ! (∙-assoc (! (f-g (f x))) (f-g (f x)) (ap (idf B) p))
             ∙ ap (λ q → q ∙ ap (idf B) p) (!-inv-l (f-g (f x))) ∙ ap-idf p ⟩
        p ∎
        where f : A → B
              f = fst e

              open is-equiv (snd e)

  equiv-ap : (x y : A) → (x == y) ≃ (–> e x == –> e y)
  equiv-ap x y = equiv (ap (–> e)) (equiv-inj e) right-inverse left-inverse

{- Equivalent types have the same truncation level -}
equiv-preserves-level : ∀ {i j} {A : Type i} {B : Type j} {n : ℕ₋₂} (e : A ≃ B)
  → (has-level n A → has-level n B)
equiv-preserves-level {n = ⟨-2⟩} e (x , p) =
  (–> e x , (λ y → ap (–> e) (p _) ∙ <–-inv-r e y))
equiv-preserves-level {n = S n} e c = λ x y →
   equiv-preserves-level (equiv-ap (e ⁻¹) x y ⁻¹) (c (<– e x) (<– e y))

{- The type-theoretic axiom of choice -}
choice : ∀ {i j k} {A : Type i} {B : A → Type j} {P : (a : A) → B a → Type k}
  → Π A (λ a → Σ (B a) (λ b → P a b)) ≃ Σ (Π A B) (λ g → Π A (λ a → P a (g a)))
choice = equiv f g (λ _ → idp) (λ _ → idp)
  where f = λ c → ((λ a → fst (c a)) , (λ a → snd (c a)))
        g = λ d → (λ a → (fst d a , snd d a))

{- Pre- and post- concatenation are equivalences -}
module _ {i} {A : Type i} {x y z : A} where

  pre∙-is-equiv : (p : x == y) → is-equiv (λ (q : y == z) → p ∙ q)
  pre∙-is-equiv p = is-eq (λ q → p ∙ q) (λ r → ! p ∙ r) f-g g-f
    where f-g : ∀ r → p ∙ ! p ∙ r == r
          f-g r = ! (∙-assoc p (! p) r) ∙ ap (λ s → s ∙ r) (!-inv-r p)

          g-f : ∀ q → ! p ∙ p ∙ q == q
          g-f q = ! (∙-assoc (! p) p q) ∙ ap (λ s → s ∙ q) (!-inv-l p)

  post∙-is-equiv : (p : y == z) → is-equiv (λ (q : x == y) → q ∙ p)
  post∙-is-equiv p = is-eq (λ q → q ∙ p) (λ r → r ∙ ! p) f-g g-f
    where f-g : ∀ r → (r ∙ ! p) ∙ p == r
          f-g r = ∙-assoc r (! p) p ∙ ap (λ s → r ∙ s) (!-inv-l p) ∙ ∙-unit-r r

          g-f : ∀ q → (q ∙ p) ∙ ! p == q
          g-f q = ∙-assoc q p (! p) ∙ ap (λ s → q ∙ s) (!-inv-r p) ∙ ∙-unit-r q

{- Homotopy fibers -}
hfiber : ∀ {i j} {A : Type i} {B : Type j} (f : A → B) (y : B) → Type (lmax i j)
hfiber {A = A} f y = Σ A (λ x → f x == y)
